Some progress on [piece_remains_valid_f]

ind/DListLowInd.fst
@@ -1116,7 +1116,14 @@ let piece_remains_valid_f (#t:Type) (h0 h1:heap) (p:piece t) :
     (ensures (piece_valid h1 p) /\ (p.phead@h0).blink == (p.phead@h1).blink) =
   let nodes = reveal p.pnodes in
   if length nodes > 1 then (
-    admit ()
+    assume (nodelist_valid h0 (fst (unsnoc nodes)));
+    unsnoc_is_last nodes;
+    // assert (Mod.loc_disjoint (Mod.loc_buffer p.ptail) (nodelist_fp0 (fst (unsnoc nodes))));
+    nodelist_remains_valid h0 h1 (Mod.loc_buffer p.ptail) (fst (unsnoc nodes));
+    assume (piece_contained h1 p);
+    assume (piece_conn h1 p);
+    // assert ((p.phead@h0).blink == (p.phead@h1).blink);
+    ()
   ) else ()
 
 (* TODO *)
